@prefix : <http://w3id.org/rsp/spin#> .
@prefix sp: <http://spinrdf.org/sp#> .
@prefix owl: <http://www.w3.org/2002/07/owl#> .
@prefix rdf: <http://www.w3.org/1999/02/22-rdf-syntax-ns#> .
@prefix rdfs: <http://www.w3.org/2000/01/rdf-schema#> .
@prefix xsd: <http://www.w3.org/2001/XMLSchema#> .

<http://w3id.org/rsp/spin>
  rdf:type owl:Ontology ;
  owl:imports <http://spinrdf.org/sp> ;
.

# Register as
:hasOutputStream
  rdf:type rdf:Property ;
  rdfs:comment "Set the name of the result stream of a query."^^xsd:string ;
  rdfs:domain sp:Query ;
  rdfs:range rdfs:Resource, sp:Variable ;
  rdfs:subPropertyOf sp:systemProperty ;
.

# Output stream operator
:hasOutputStreamOperator
  rdf:type rdf:Property ;
  rdfs:comment "Property to set the output stream operator of a query."^^xsd:string ;
  rdfs:domain sp:Query ;
  rdfs:range :OutputStreamOperator ;
  rdfs:subPropertyOf sp:systemProperty ;
.
:OutputStreamOperator
  rdfs:comment "Stream output operator."^^xsd:string ;
  rdf:type rdfs:Class ;
  rdfs:subClassOf sp:Element ;
.
:Dstream
  rdf:type rdfs:Class ;
  rdfs:comment "States that the output stream operator is Dstream (i.e., return results that are in the previous window but not the current one)."^^xsd:string ;
  rdfs:subClassOf :OutputStreamOperator ;
.
:Istream
  rdf:type rdfs:Class ;
  rdfs:comment "States that the output stream operator is Istream (i.e., return results that are in the current window but were not present in the previous one)."^^xsd:string ;
  rdfs:subClassOf :OutputStreamOperator ;
.
:Rstream
  rdf:type rdfs:Class ;
  rdfs:comment "States that the output stream operator is Rstream (i.e., return all results that are in the current window)."^^xsd:string ;
  rdfs:subClassOf :OutputStreamOperator ;
.

# Named window
:fromNamedWindow
  rdf:type rdf:Property ;
  rdfs:comment "Property to define a named window for a query."^^xsd:string ;
  rdfs:domain sp:Query ;
  rdfs:range :NamedWindow ;
  rdfs:subPropertyOf sp:systemProperty ;
.
:NamedWindow
  rdf:type rdfs:Class ;
  rdfs:comment "A named window over a stream."^^xsd:string ;
  rdfs:subClassOf sp:ElementGroup ;
.
:windowNameNode
  rdf:type rdf:Property ;
  rdfs:comment "Property to set the name of a window."^^xsd:string ;
  rdfs:range rdfs:Resource ;
  rdfs:subPropertyOf sp:systemProperty ;
.
:streamUri
  rdf:type rdf:Property ;
  rdfs:comment "Property to set the stream of a window."^^xsd:string ;
  rdfs:domain :NamedWindow ;
  rdfs:range rdfs:Resource, sp:Variable ;
  rdfs:subPropertyOf sp:systemProperty ;
.
:windowUri
  rdf:type rdf:Property ;
  rdfs:comment "Property to set the name of a window."^^xsd:string ;
  rdfs:domain :NamedWindow ;
  rdfs:range rdfs:Resource ;
  rdfs:subPropertyOf sp:systemProperty ;
.

# Logical window
:LogicalWindow
  rdf:type rdfs:Class ;
  rdfs:comment "A logical window defined using range and step expressed as durations."^^xsd:string ;
  rdfs:subClassOf :NamedWindow ;
.
:logicalRange
  rdf:type rdf:Property ;
  rdfs:comment "Property to set the duration of a logical range."^^xsd:string ;
  rdfs:domain :LogicalWindow ;
  rdfs:range xsd:duration, sp:Variable ;
  rdfs:subPropertyOf sp:systemProperty ;
.
:logicalStep
  rdf:type rdf:Property ;
  rdfs:comment "Property to set the duration of a logical step."^^xsd:string ;
  rdfs:domain :LogicalPastWindow, :LogicalWindow ;
  rdfs:range xsd:duration ;
  rdfs:range sp:Variable ;
  rdfs:subPropertyOf sp:systemProperty ;
.

# Logical past window
:LogicalPastWindow
  rdf:type rdfs:Class ;
  rdfs:comment "A logical past window defined using a lower and an upper time bound."^^xsd:string ;
  rdfs:subClassOf :NamedWindow ;
.
:from
  rdf:type rdf:Property ;
  rdfs:comment "Property to set the start of a window relative to the current time."^^xsd:string ;
  rdfs:domain :LogicalPastWindow ;
  rdfs:range xsd:duration, sp:Variable ;
  rdfs:subPropertyOf sp:systemProperty ;
.
:to
  rdf:type rdf:Property ;
  rdfs:comment "Property to set the end of a window relative to the current time."^^xsd:string ;
  rdfs:domain :LogicalPastWindow ;
  rdfs:range xsd:duration, sp:Variable ;
  rdfs:subPropertyOf sp:systemProperty ;
.

# Physical window
:PhysicalWindow
  rdf:type rdfs:Class ;
  rdfs:comment "A physical window defined using size and step expressed as number elements."^^xsd:string ;
  rdfs:subClassOf :NamedWindow ;
.
:physicalRange
  rdf:type rdf:Property ;
  rdfs:comment "Property to set the size of a window expressed as number of elements."^^xsd:string ;
  rdfs:domain :PhysicalWindow ;
  rdfs:range xsd:integer, sp:Variable ;
  rdfs:subPropertyOf sp:systemProperty ;
.
:physicalStep
  rdf:type rdf:Property ;
  rdfs:comment "Property to set the step of a window expressed as number of elements."^^xsd:string ;
  rdfs:domain :PhysicalWindow ;
  rdfs:range xsd:integer, sp:Variable ;
  rdfs:subPropertyOf sp:systemProperty ;
.
